theories/stdpp_extra.v
@@ -604,6 +604,20 @@ Proof.
   - intros l2. cbn [list_difference list_to_set]. destruct (decide_rel elem_of a l2); set_solver.
 Qed.
 
+Definition prod_op {A B : Type} :=
+  λ (o1 : option A) (o2 : option B),
+    match o1 with
+    | Some b =>
+        match o2 with
+        | Some c => Some (b,c)
+        | None => None
+        end
+    | None => None
+    end.
+
+Definition prod_merge {A B C : Type} `{Countable A} : gmap A B → gmap A C → gmap A (B * C) :=
+  λ m1 m2, merge prod_op m1 m2.
+
 (* creates a gmap with domain from the list, all pointing to a default value *)
 Fixpoint create_gmap_default {K V : Type} `{Countable K}
          (l : list K) (d : V) : gmap K V :=
@@ -646,6 +660,33 @@ Proof.
   - cbn. rewrite dom_empty_L //.
   - cbn [create_gmap_default list_to_set]. rewrite dom_insert_L // IHl //.
 Qed.
+
+Lemma create_gmap_default_lookup_None {K V : Type} `{Countable K}
+  (l : list K) (d : V) (k : K) :
+  k ∉ l →
+  (create_gmap_default l d) !! k = None.
+Proof.
+  intros Hk.
+  induction l;auto.
+  simpl. apply not_elem_of_cons in Hk as [Hne Hk].
+  rewrite lookup_insert_ne//. apply IHl. auto.
+Qed.
+Lemma create_gmap_default_permutation {K V : Type} `{Countable K}
+  (l l' : list K) (d : V) :
+  l ≡ₚl' →
+  (create_gmap_default l d) = (create_gmap_default l' d).
+Proof.
+  intros Hperm.
+  apply map_eq. intros k.
+  destruct (decide (k ∈ l)).
+  - assert (k ∈ l') as e';[rewrite -Hperm;auto|].
+    apply (create_gmap_default_lookup _ d) in e as ->.
+    apply (create_gmap_default_lookup _ d) in e' as ->. auto.
+  - assert (k ∉ l') as e';[rewrite -Hperm;auto|].
+    apply (create_gmap_default_lookup_None _ d) in n as ->.
+    apply (create_gmap_default_lookup_None _ d) in e' as ->. auto.
+Qed.
+
 
 Lemma map_filter_sub :
 ∀ (K : Type) (M : Type → Type) (H : FMap M) (H0 :
@@ -977,3 +1018,102 @@ Proof.
     simpl. rewrite rev_unit. rewrite rev_involutive. rewrite -Hsome /=.
     f_equiv. rewrite firstn_all. auto.
 Qed.
+
+Lemma pair_eq_inv {A B} {y u : A} {z t : B} {x} :
+    x = (y, z) -> x = (u, t) ->
+    y = u ∧ z = t.
+Proof. intros ->. inversion 1. auto. Qed.
+
+(* TODO: integrate into stdpp? *)
+Tactic Notation "simplify_pair_eq" :=
+  repeat
+    lazymatch goal with
+    | H1 : ?x = (?y, ?z), H2 : ?x = (?u, ?t) |- _ =>
+      assert (y = u ∧ z = t) as [? ?] by (exact (pair_eq_inv H1 H2)); clear H2
+    | H1 : (?y, ?z) = ?x, H2 : ?x = (?u, ?t) |- _ =>
+      assert (y = u ∧ z = t) as [? ?] by (exact (pair_eq_inv (eq_sym H1) H2)); clear H2
+    | H1 : ?x = (?y, ?z), H2 : (?u, ?t) = ?x |- _ =>
+      assert (y = u ∧ z = t) as [? ?] by (exact (pair_eq_inv H1 (eq_sym H2))); clear H2
+    | H1 : (?y, ?z) = ?x, H2 : (?u, ?t) = ?x |- _ =>
+      assert (y = u ∧ z = t) as [? ?] by (exact (pair_eq_inv (eq_sym H1) (eq_sym H2))); clear H2
+    | |- _ => progress simplify_eq
+    end.
+
+(*----------------------- FIXME TEMPORARY ------------------------------------*)
+(* This is a copy-paste from stdpp (fin_maps.v), plus a fix to avoid using
+   "rewrite .. by .." that is not available when using ssreflect's rewrite. *)
+(* TODO: upstream the fix into stdpp, and remove the code below whenever we
+   upgrade to a version of stdpp that includes it *)
+
+Tactic Notation "simpl_map" "by" tactic3(tac) := repeat
+  match goal with
+  | H : context[ ∅ !! _ ] |- _ => rewrite lookup_empty in H
+  | H : context[ (<[_:=_]>_) !! _ ] |- _ =>
+    rewrite lookup_insert in H || (rewrite lookup_insert_ne in H; [| by tac])
+  | H : context[ (alter _ _ _) !! _] |- _ =>
+    rewrite lookup_alter in H || (rewrite lookup_alter_ne in H; [| by tac])
+  | H : context[ (delete _ _) !! _] |- _ =>
+    rewrite lookup_delete in H || (rewrite lookup_delete_ne in H; [| by tac])
+  | H : context[ {[ _ := _ ]} !! _ ] |- _ =>
+    rewrite lookup_singleton in H || (rewrite lookup_singleton_ne in H; [| by tac])
+  | H : context[ (_ <$> _) !! _ ] |- _ => rewrite lookup_fmap in H
+  | H : context[ (omap _ _) !! _ ] |- _ => rewrite lookup_omap in H
+  | H : context[ lookup (A:=?A) ?i (?m1 ∪ ?m2) ] |- _ =>
+    let x := fresh in evar (x:A);
+    let x' := eval unfold x in x in clear x;
+    let E := fresh in
+    assert ((m1 ∪ m2) !! i = Some x') as E by (clear H; by tac);
+    rewrite E in H; clear E
+  | |- context[ ∅ !! _ ] => rewrite lookup_empty
+  | |- context[ (<[_:=_]>_) !! _ ] =>
+    rewrite lookup_insert || (rewrite lookup_insert_ne; [| by tac])
+  | |- context[ (alter _ _ _) !! _ ] =>
+    rewrite lookup_alter || (rewrite lookup_alter_ne; [| by tac])
+  | |- context[ (delete _ _) !! _ ] =>
+    rewrite lookup_delete || (rewrite lookup_delete_ne; [| by tac])
+  | |- context[ {[ _ := _ ]} !! _ ] =>
+    rewrite lookup_singleton || (rewrite lookup_singleton_ne; [| by tac])
+  | |- context[ (_ <$> _) !! _ ] => rewrite lookup_fmap
+  | |- context[ (omap _ _) !! _ ] => rewrite lookup_omap
+  | |- context [ lookup (A:=?A) ?i ?m ] =>
+    let x := fresh in evar (x:A);
+    let x' := eval unfold x in x in clear x;
+    let E := fresh in
+    assert (m !! i = Some x') as E by tac;
+    rewrite E; clear E
+  end.
+
+Tactic Notation "simpl_map" := simpl_map by eauto with simpl_map map_disjoint.
+
+Tactic Notation "simplify_map_eq" "by" tactic3(tac) :=
+  decompose_map_disjoint;
+  repeat match goal with
+  | _ => progress simpl_map by tac
+  | _ => progress simplify_eq/=
+  | _ => progress simpl_option by tac
+  | H : {[ _ := _ ]} !! _ = None |- _ => rewrite lookup_singleton_None in H
+  | H : {[ _ := _ ]} !! _ = Some _ |- _ =>
+    rewrite lookup_singleton_Some in H; destruct H
+  | H1 : ?m1 !! ?i = Some ?x, H2 : ?m2 !! ?i = Some ?y |- _ =>
+    let H3 := fresh in
+    feed pose proof (lookup_weaken_inv m1 m2 i x y) as H3; [done|by tac|done|];
+    clear H2; symmetry in H3
+  | H1 : ?m1 !! ?i = Some ?x, H2 : ?m2 !! ?i = None |- _ =>
+    let H3 := fresh in
+    apply (lookup_weaken _ m2) in H1; [congruence|by tac]
+  | H : ?m ∪ _ = ?m ∪ _ |- _ =>
+    apply map_union_cancel_l in H; [|by tac|by tac]
+  | H : _ ∪ ?m = _ ∪ ?m |- _ =>
+    apply map_union_cancel_r in H; [|by tac|by tac]
+  | H : {[?i := ?x]} = ∅ |- _ => by destruct (map_non_empty_singleton i x)
+  | H : ∅ = {[?i := ?x]} |- _ => by destruct (map_non_empty_singleton i x)
+  | H : ?m !! ?i = Some _, H2 : ?m !! ?j = None |- _ =>
+     unless (i ≠ j) by done;
+     assert (i ≠ j) by (by intros ?; simplify_eq)
+  end.
+Tactic Notation "simplify_map_eq" "/=" "by" tactic3(tac) :=
+  repeat (progress csimpl in * || simplify_map_eq by tac).
+Tactic Notation "simplify_map_eq" :=
+  simplify_map_eq by eauto with simpl_map map_disjoint.
+Tactic Notation "simplify_map_eq" "/=" :=
+  simplify_map_eq/= by eauto with simpl_map map_disjoint.
