theories/rules/rules_Get.v
@@ -2,7 +2,7 @@ From iris.base_logic Require Export invariants gen_heap.
 From iris.program_logic Require Export weakestpre ectx_lifting.
 From iris.proofmode Require Import proofmode.
 From iris.algebra Require Import frac.
-From cap_machine Require Export rules_base.
+From cap_machine Require Export rules_base stdpp_extra.
 
 Section cap_lang_rules.
   Context `{memG Σ, regG Σ}.
@@ -12,10 +12,12 @@ Section cap_lang_rules.
   Implicit Types c : cap_lang.expr.
   Implicit Types a b : Addr.
   Implicit Types r : RegName.
-  Implicit Types v : cap_lang.val.
-  Implicit Types w : Word.
-  Implicit Types reg : gmap RegName Word.
-  Implicit Types ms : gmap Addr Word.
+  Implicit Types v : Version.
+  Implicit Types lw: LWord.
+  Implicit Types reg : Reg.
+  Implicit Types lregs : LReg.
+  Implicit Types mem : Mem.
+  Implicit Types lmem : LMem.
 
   (* Generalized denote function, since multiple cases result in similar success *)
   Definition denote (i: instr) (w : Word): option Z :=
